fix comments to fit report

Paxos/Prop.lean
@@ -6,58 +6,49 @@ open Paxos.Spec
 variable (sent sent' : Set Message)
 variable (Quorums : Set (Set Acceptor))
 
-/--
-VotedForIn(a, v, b) means that acceptor a has sent some 2b message m with m.val equal to v and m.bal equal to b. This specifies that acceptor a has voted the pair ⟨v, b⟩.
--/
+/-- VotedForIn(a, v, b) means that acceptor a has sent some 2b message m with m.val
+equal to v and m.bal equal to b. This specifies that acceptor a has voted the pair ⟨v, b⟩.-/
 def VotedForIn (a : Acceptor) (v : Value) (b : Ballot) : Prop :=
   ∃ m ∈ sent, m = Message.twob b v a
 
-/--
-ChosenIn(v, b) means that every acceptor in some quorum Q has voted the pair hv, bi.
--/
+/-- ChosenIn(v, b) means that every acceptor in some quorum Q has voted the pair hv, bi. -/
 def ChosenIn (v: Value) (b: Ballot) : Prop :=
   ∃ Q ∈ Quorums, ∀ a ∈ Q, VotedForIn sent a v b
 
-/--
-Chosen(v) means that for some ballot b, ChosenIn(v, b) holds.
--/
+/-- Chosen(v) means that for some ballot b, ChosenIn(v, b) holds. -/
 def Chosen (v : Value) : Prop :=
   ∃ b : Ballot, ChosenIn sent Quorums v b
 
-/--
-WontVoteIn(a, b) means that acceptor a has seen a higher ballot than b, and did not and will not vote any value with ballot b.
--/
+/-- WontVoteIn(a, b) means that acceptor a has seen a higher ballot than b,
+and did not and will not vote any value with ballot b. -/
 def WontVoteIn (a : Acceptor) (b : Ballot) : Prop :=
   (∀ v : Value, ¬VotedForIn sent a v b) ∧
   (∃ m ∈ sent, match m with
-    | Message.oneb b' _ _ a' => a' = a ∧ b' > b           -- either a 1b message with ballot greater than b
-    | Message.twob b' _ a'   => a' = a ∧ b' > b           -- or a 2b message with ballot greater than b
+    | Message.oneb b' _ _ a' => a' = a ∧ b' > b  -- 1b message with ballot greater than b
+    | Message.twob b' _ a'   => a' = a ∧ b' > b  -- 2b message with ballot greater than b
     | _                      => false)
 
-/--
-SafeAt(v, b) means that no value except perhaps v has been or will be chosen in any ballot lower than b.
--/
+/-- SafeAt(v, b) means that no value except perhaps v has been or will be chosen
+in any ballot lower than b. -/
 def SafeAt (v : Value) (b : Ballot) : Prop :=
   ∀ b2 < b,
     ∃ Q ∈ Quorums,
       ∀ a ∈ Q, VotedForIn sent a v b2 ∨ WontVoteIn sent a b2
 
-/--
-MsgInv defines properties satisfied by the contents of messages, for 1b, 2a, and 2b messages.
--/
+/-- Message invariants for 1b, 2a, and 2b messages. -/
 def MsgInv : Prop :=
   ∀ m ∈ sent, match m with
-    | Message.oneb b maxVBal maxVal a => (
-      match maxVBal, maxVal with                             -- ! in the TLA proof this is matched with ballot number (-1) and otherwise. We match it with both, and added another invariant that is, when one of them is none, the other is also none.
-        | some rbal, some rval => VotedForIn sent a rval rbal
-        | option_rbal, option_rval => option_rbal = none ∧ option_rval = none)          -- ADDED in the Lean proof
-      ∧
-      (∀ (b' : Ballot), ((b' ≥ maxVBal + (1: Nat)) ∧ (b' < b)) → ¬ (∃ v : Value, VotedForIn sent a v b')) -- This works even if `maxVBal` is none, because we defined `LE` for `Ballot` and `Option Ballot`, see Spec.lean
-    | Message.twoa b v =>   (SafeAt sent Quorums v b) -- this only applies to 2a messages
-                          ∧ (∀ m2 ∈ sent, match m2 with
-                              | Message.twoa b' _ => (b' = b → m2 = m)
-                              | _                  => True)
-    | Message.twob (some b) (some v) _ => Message.twoa b v ∈ sent
+    | Message.oneb b maxVBal maxVal a  =>
+        (match maxVBal, maxVal with
+          | some rbal, some rval         => VotedForIn sent a rval rbal
+          | option_rbal, option_rval     => option_rbal = none ∧ option_rval = none)
+      ∧ (∀ (b' : Ballot), (b' ≥ (maxVBal + (1: Nat)) ∧ (b' < b))
+          → ¬(∃ v : Value, VotedForIn sent a v b'))
+    | Message.twoa b v                 =>   (SafeAt sent Quorums v b)
+                                          ∧ (∀ m2 ∈ sent, match m2 with
+                                             | Message.twoa b' _ => (b' = b → m2 = m)
+                                             | _                 => True)
+    | Message.twob (some b) (some v) _ =>   Message.twoa b v ∈ sent
     | _ => True
 
 def Consistency : Prop :=
