Paxos/Spec.lean
@@ -7,15 +7,13 @@ open Classical
 /-- Types Definition
     For simplicity, we hardwire Acceptor and Value to be String (instead of Type).
     We keep Ballot the same as TLA+ spec, which is natural numbers.
-    For the empty ballot (defined as -1 in the TLAPS proof), we use none (Option Ballot).
- -/
+    For the empty ballot (defined as -1 in the TLAPS proof), we use none (Option Ballot).-/
 abbrev Acceptor := String
 abbrev Value := String
 abbrev Ballot := Nat
 
-/--
-  Since we map the empty ballot (-1) to none, need to define `+` between Option Ballot and Nat.
--/
+/-- Since we map the empty ballot (-1) to none,
+    need to define `+` between Option Ballot and Nat. -/
 instance : HAdd (Option Ballot) Nat (Option Ballot) where
   hAdd
     | none,    0          => none         -- -1 + 0     = -1
@@ -30,7 +28,8 @@ instance : HAdd (Option Ballot) Nat (Option Ballot) where
 -- #eval (some 0: Option Ballot) ≤ (some 1: Option Ballot)
 -- #eval (none: Option Ballot) + 1 ≤ (none: Option Ballot)
 
--- Minimal example, I was trying to prove this using linarith but it didn't work. This is used to prove the inductiveness of Phase 2a.
+-- Minimal example for ballot comparison (used to prove the inductiveness of Phase 2a.)
+-- linarith didn't work.
 example {b b1: Ballot} (h1: b1 ≤ b) (h2: b ≤ b1 - 1) (h3: b1 > 0) : False := by
   have h2' : b < b1 := by exact (Nat.lt_iff_le_pred h3).mpr h2
   have hf : b1 < b1 := by exact Nat.lt_of_le_of_lt h1 h2'
@@ -41,12 +40,15 @@ theorem ballot_none_plus_one_leq_ballot {b : Ballot} : (none : Option Ballot) + 
   dsimp [HAdd.hAdd]
   exact Nat.zero_le b
 
-/- Message is defined as an inductive type -/
+/-- Message is defined as an inductive type -/
+--! in oneb `maxVBal` and `maxVal` are defined to be `Option` type.
+--! `bal` and `val` in `twob` are also defined to be `Option` type, this is a modification
+--! from the TLA+ spec to ensure type consistency with `max_prop`.
 inductive Message where
 | onea  (bal : Ballot)
-| oneb  (bal : Ballot) (maxVBal : Option Ballot) (maxVal : Option Value) (acc : Acceptor) -- `maxVBal` and `maxVal` are defined to be Option, they correspond to no previous twob messages.
+| oneb  (bal : Ballot) (maxVBal : Option Ballot) (maxVal : Option Value) (acc : Acceptor)
 | twoa  (bal : Ballot) (val : Value)
-| twob  (bal : Option Ballot) (val : Option Value) (acc : Acceptor)                       -- Both `bal` and `val` are Option type because `max_prop`. This is a modification from the TLA proof.
+| twob  (bal : Option Ballot) (val : Option Value) (acc : Acceptor)
 deriving DecidableEq, Repr
 
 /-  Line 16 - 18
@@ -74,41 +76,41 @@ def Send (m : Message) (sent : Set Message) := sent ∪ {m}
 Init == sent = {} -/
 def Init : Prop := sent = ∅
 
-/--
-Phase 1a: A 1a message with ballot b is sent by some proposer (to all processes).
--/
+/-- Phase 1a: A 1a message with ballot b is sent by some proposer (to all processes). -/
 @[simp]
 def Phase1a (b : Ballot) : Prop :=
   sent' = Send (Message.onea b) sent
 
 /-- Get the maximum ballot and value that an acceptor has voted for.
 
-However, instead of returning a tuple for the ballot and value, we return a set of 2b messages.
+instead of returning a tuple for the ballot and value, return a set of 2b messages.
 Note: last_voted(a) is used in the [github repo](https://github.com/DistAlgo/proofs/blob/master/basic-paxos/PaxosHistVarNFM18.tla#L47). However, in the paper (https://arxiv.org/pdf/1802.09687), the name is max_prop. Here we use max_prop because it is more informative.
 -/
 def max_prop (a : Acceptor): Set Message :=
-  let twobs := {m ∈ sent | ∃ (b: Ballot) (v: Value), m = Message.twob b v a}          -- The twob messages should have concrete ballot and value, not Option type. We explicitly write out the types.
+  let twobs := {m ∈ sent | ∃ (b: Ballot) (v: Value), m = Message.twob b v a}
   if twobs ≠ ∅ then
-    { m₁ ∈ twobs | ∀m₂ ∈ twobs, ∃ (b₁ b₂: Ballot) (v₁ v₂: Value),                     -- Same as above
-      m₁ = Message.twob b₁ v₁ a ∧ m₂ = Message.twob b₂ v₂ a ∧ b₁ ≥ b₂}
-  else {Message.twob none none a}                                                     -- For -1 ballot, we use `none`. At the same time, returning `none` as the value.
+      {m₁ ∈ twobs | ∀m₂ ∈ twobs, ∃ (b₁ b₂: Ballot) (v₁ v₂: Value),
+                      m₁ = Message.twob b₁ v₁ a ∧ m₂ = Message.twob b₂ v₂ a ∧ b₁ ≥ b₂}
+  else {Message.twob none none a}  -- For -1 ballot, we use `none`.
 
 /-- Phase 1b: For an acceptor a, if there is a 1a message m with ballot m.bal that is higher than the highest it
 has seen, a sends a 1b message with m.bal alongwith the highest-numbered pair it has voted for.
 
-The If-then-else is used to simplify the definition, because we need to assert in the case of the guard not being satisfied, `sent' = sent`.
+The If-then-else is used to simplify the definition, because we need to assert in the case of the guard not
+being satisfied, `sent' = sent`.
 
-In first order logic we would write this as: `(A → B) ∧ (¬A → C)`, where `A` is the guard condition, `B` is the action to be taken if the guard is satisfied, and `C` is the action to be taken if the guard is not satisfied. In Lean, we can use `if-then-else` to express this in a more compact way, so `A` only appears once: `if A then B else C`.
--/
+In first order logic we would write this as: `(A → B) ∧ (¬A → C)`, where `A` is the guard condition, `B` is the action
+to be taken if the guard is satisfied, and `C` is the action to be taken if the guard is not satisfied.
+We use `if-then-else` to express this in a more compact way, so `A` only appears once: `if A then B else C`. -/
 def Phase1b (a : Acceptor) : Prop :=
   ∃ m ∈ sent, ∃r ∈ max_prop sent a,
     match m, r with
-    | Message.onea b, Message.twob rbal rval _a =>          -- rbal and rval are Option type, they could both be none.
+    | Message.onea b, Message.twob rbal rval _a =>
        if (∀m2 ∈ sent, match m2 with
        | Message.oneb b2 _ _ a' => (a' = a) → (b > b2)
        | Message.twob b2 _ a' => (a' = a) → (b > b2)
        | _ => True)
-       then sent' = Send (Message.oneb b rbal rval a) sent  -- rbal and rval are Option type, they could both be none.
+       then sent' = Send (Message.oneb b rbal rval a) sent
        else sent' = sent
     | _, _ => False
 
@@ -116,28 +118,35 @@ def Phase1b (a : Acceptor) : Prop :=
 messages with ballot b, a proposer sends a 2a message with ballot b and value v, where v is the value with
 the highest ballot in S, or is any value in V if no acceptor that responded in S has voted for anything.
 
-The choice of using if-then-else if to make the definition shorter, similar to the Phase1b definition. However, we have nested guard conditions, so multiple if-then-else are used.
--/
+The choice of using if-then-else if to make the definition shorter, similar to the Phase1b definition. However, we have nested guard conditions, so multiple if-then-else are used. -/
 def Phase2a (b : Ballot) : Prop :=
   if (¬∃ m ∈ sent, match m with
                 | Message.twoa b' _ => b' = b
                 | _                 => False)
-  then
-    if φ : ∃ (v : Value) (Q : Set Acceptor) (S : Set Message), Q ∈ Quorums ∧ S ⊆ { m ∈ sent | match m with | Message.oneb b' _ _ _ => b' = b | _ => False}  -- S is the set of 1b messages with ballot b
-      ∧ (∀ a ∈ Q, ∃ m ∈ S, match m with | Message.oneb _ _ _ a' => a' = a | _ => False)         -- for all acceptors in Q, there is a corresponding 1b message in S.
-      ∧ ((∀ m ∈ S, match m with | Message.oneb _ maxVBal _ _ => maxVBal = none | _ => True)     -- for all 1b messages, either that maxVal is -1 (no acceptor has voted for anything)
-          ∨ ∃ (c : Ballot), 0 ≤ c ∧ c ≤ b - (1 : Nat)                                             -- or there is a 1b message with ballot c (the 'highest ballot') that is less than b
-              ∧ (∀ m ∈ S, match m with | Message.oneb _ maxVBal _ _ => maxVBal ≤ c | _ => True)   -- and for all 1b messages, the maxV is less than or equal to c
-              ∧ (∃ m ∈ S, match m with | Message.oneb _ maxVBal maxVal _ => maxVBal = c ∧ maxVal = v | _ => False)) -- and there is a 1b message with ballot c and value v
-    then let v := choose φ; sent' = Send (Message.twoa b v) sent                                -- because `φ` is true, we can choose such value `v`.
-    else
-      sent' = sent
-  else
-    sent' = sent
+  then if φ : ∃ (v : Value) (Q : Set Acceptor) (S : Set Message),
+              Q ∈ Quorums
+            ∧ S ⊆ { m ∈ sent | match m with
+                               | Message.oneb b' _ _ _ => b' = b
+                               | _ => False}
+      ∧ (∀ a ∈ Q, ∃ m ∈ S, match m with
+                           | Message.oneb _ _ _ a' => a' = a
+                           | _ => False)
+      ∧ ((∀ m ∈ S, match m with
+                   | Message.oneb _ maxVBal _ _ => maxVBal = none
+                   | _ => True)
+        ∨ ∃ (c : Ballot), 0 ≤ c ∧ c ≤ b - (1 : Nat)
+            ∧ (∀ m ∈ S, match m with
+                        | Message.oneb _ maxVBal _ _ => maxVBal ≤ c
+                        | _ => True)
+            ∧ (∃ m ∈ S, match m with
+                        | Message.oneb _ maxVBal maxVal _ => maxVBal = c ∧ maxVal = v
+                        | _ => False))
+        then let v := choose φ; sent' = Send (Message.twoa b v) sent
+    else sent' = sent
+  else sent' = sent
 
-/-- Phase 2b: For an acceptor a, if there is a 2a message m with ballot m.bal that is higher than or equal to the
-highest it has seen, a sends a 2b message with m.bal and m.val.
--/
+/-- Phase 2b: For an acceptor a, if there is a 2a message m with ballot m.bal that is higher
+than or equal to the highest it has seen, a sends a 2b message with m.bal and m.val. -/
 def Phase2b (a : Acceptor) : Prop :=
   ∃ m ∈ sent, match m with
     | Message.twoa b v =>
@@ -149,21 +158,21 @@ def Phase2b (a : Acceptor) : Prop :=
       else sent' = sent
     | _ => sent' = sent
 
-/--
-Next == \/ \E b \in Ballots : Phase1a(b) \/ Phase2a(b)
-        \/ \E a \in Acceptors : Phase1b(a) \/ Phase2b(a)
-** The lean code below is equivalent to the above definition, written in a more proof-friendly way for rcases to work
--/
+/-- Next == \/ \E b \in Ballots : Phase1a(b) \/ Phase2a(b)
+        \/ \E a \in Acceptors : Phase1b(a) \/ Phase2b(a) -/
+--! equvilant to the TLA+ definition, written this way for convienience of `rcases`.
 def Next := (∃b, Phase1a sent sent' b ∨ Phase2a Quorums sent sent' b)
           ∨ (∃a, Phase1b sent sent' a ∨ Phase2b sent sent' a)
 
 /--
-The Specification of Paxos. `σ` represents the trace of the system, which is mapping between `ℕ` and `Set Message`.
-
-The initial state is `Init (σ 0)`, and the next state is defined by `Next Quorums (σ i) (σ (i+1))` for all `i`. The disjunction allows for the stuttering step.
-
-This is Spec == Init /\ [][Next]_vars. Naming it PaxosSpec to avoid confusion with the `Spec` namespace.
--/
+    The Specification of Paxos. This is `Spec == Init /\ [][Next]_vars` in TLA+.
+    `σ` represents the trace of the system, which is mapping from `ℕ` to `Set Message`.
+    1. The initial state is `Init (σ 0)`
+    2. The next state is defined by the relation
+      `Next Quorums (σ i) (σ (i+1)) ∨ (σ i) = (σ (i+1))`.
+    3. Always operator is modeled by the universal quantification over all `i`.
+    4. `(σ i) = (σ (i+1))` in the second part of the disjunction models stuttering steps.
+    It is named `PaxosSpec` to avoid name clashes with the `Spec` namespace. -/
 def PaxosSpec (σ : ℕ → Set Message) : Prop :=
   Init (σ 0) ∧ (∀ i, Next Quorums (σ i) (σ (i+1)) ∨ (σ i) = (σ (i+1)))
 
